ironfleet/src/Dafny/Distributed/Impl/Lock/Host.i.dfy
@@ -1,9 +1,9 @@
-include "../../Common/Framework/Host.s.dfy"
+// include "../../Common/Framework/Host.s.dfy"
 include "../../Common/Collections/Sets.i.dfy"
 include "NodeImpl.i.dfy"
 include "CmdLineParser.i.dfy"
 
-module Host_i refines Host_s {
+module Host_i {
     import opened Collections__Sets_i
     import opened Protocol_Node_i
     import opened NodeImpl_i
@@ -12,14 +12,21 @@ module Host_i refines Host_s {
     import opened Types_i
     import opened Impl_Node_i
     import opened NetLock_i
-    export Spec
-        provides Native__Io_s, Environment_s, Native__NativeTypes_s
-        provides HostState
-        provides ConcreteConfiguration
-        provides HostInit, HostNext, ConcreteConfigInit, HostStateInvariants
-        provides ConcreteConfigToServers, ParseCommandLineConfiguration, ArbitraryObject
-        provides HostInitImpl, HostNextImpl
-    export All reveals *
+    // export Spec
+    //     provides Native__Io_s, Environment_s, Native__NativeTypes_s
+    //     provides HostState
+    //     provides ConcreteConfiguration
+    //     provides HostInit, HostNext, ConcreteConfigInit, HostStateInvariants
+    //     provides ConcreteConfigToServers, ParseCommandLineConfiguration, ArbitraryObject
+    //     provides HostInitImpl, HostNextImpl
+    // export All reveals *
+
+    import opened Native__Io_s
+    import opened Environment_s 
+    import opened Native__NativeTypes_s
+
+    // Tony: this file originally refined Host_s, but the refinement crashes dafny 4.2 (and also 4.4)
+    ghost predicate ArbitraryObject(o:object) { true }
 
     datatype CScheduler = CScheduler(ghost node:Node, node_impl:NodeImpl)
 
@@ -27,6 +34,7 @@ module Host_i refines Host_s {
     type ConcreteConfiguration = Config
 
     ghost predicate HostStateInvariants(host_state:HostState, env:HostEnvironment)
+        reads *
     {
       && host_state.node_impl.Valid() 
       && host_state.node_impl.Env() == env
@@ -34,6 +42,7 @@ module Host_i refines Host_s {
     }
 
     ghost predicate HostInit(host_state:HostState, config:ConcreteConfiguration, id:EndPoint)
+        reads *
     {
       && host_state.node_impl.Valid()
       && host_state.node_impl.node.config == config
@@ -72,6 +81,20 @@ module Host_i refines Host_s {
       ok:bool,
       host_state:HostState
       )
+        requires env.Valid()
+        requires env.ok.ok()
+        requires netc.IsOpen()
+        requires netc.env == env
+        requires ValidPhysicalAddress(EndPoint(netc.MyPublicKey()))
+        modifies set x:object | ArbitraryObject(x)     // Everything!
+        ensures  ok ==> env.Valid() && env.ok.ok()
+        ensures  ok ==> HostStateInvariants(host_state, env)
+        ensures  ok ==> var id := EndPoint(netc.MyPublicKey());
+                        var config := ParseCommandLineConfiguration(args);
+                        && id in ConcreteConfigToServers(config)
+                        && ConcreteConfigInit(config)
+                        && HostInit(host_state, config, id)
+        ensures  env.net.history() == old(env.net.history()) // Prohibit HostInitImpl from sending (and receiving) packets
     {
         var my_index;
         var node_impl := new NodeImpl();
@@ -97,18 +120,18 @@ module Host_i refines Host_s {
     }
 
     ghost method RemoveRecvs(events:seq<NetEvent>) returns (recvs:seq<NetEvent>, rest:seq<NetEvent>) 
-        ensures forall e :: e in recvs ==> e.LIoOpReceive?;
-        ensures events == recvs + rest;
-        ensures rest != [] ==> !rest[0].LIoOpReceive?;
+        ensures forall e :: e in recvs ==> e.LIoOpReceive?
+        ensures events == recvs + rest
+        ensures rest != [] ==> !rest[0].LIoOpReceive?
     {
         recvs := [];
         rest := [];
 
         var i := 0;
         while i < |events| 
-            invariant 0 <= i <= |events|;
-            invariant forall e :: e in recvs ==> e.LIoOpReceive?;
-            invariant recvs == events[0..i];
+            invariant 0 <= i <= |events|
+            invariant forall e :: e in recvs ==> e.LIoOpReceive?
+            invariant recvs == events[0..i]
         {
             if !events[i].LIoOpReceive? {
                 rest := events[i..];
@@ -125,10 +148,10 @@ module Host_i refines Host_s {
     }
 
     lemma RemainingEventsAreSends(events:seq<NetEvent>)
-        requires NetEventsReductionCompatible(events);
-        requires |events| > 0;
-        requires !events[0].LIoOpReceive?;
-        ensures  forall e :: e in events[1..] ==> e.LIoOpSend?;
+        requires NetEventsReductionCompatible(events)
+        requires |events| > 0
+        requires !events[0].LIoOpReceive?
+        ensures  forall e :: e in events[1..] ==> e.LIoOpSend?
     {
         if |events| == 1 {
         } else {
@@ -138,10 +161,10 @@ module Host_i refines Host_s {
     }
 
     ghost method PartitionEvents(events:seq<NetEvent>) returns (recvs:seq<NetEvent>, clocks:seq<NetEvent>, sends:seq<NetEvent>)
-        requires NetEventsReductionCompatible(events);
-        ensures  events == recvs + clocks + sends;
-        ensures  EventsConsistent(recvs, clocks, sends);
-        ensures  |clocks| <= 1;
+        requires NetEventsReductionCompatible(events)
+        ensures  events == recvs + clocks + sends
+        ensures  EventsConsistent(recvs, clocks, sends)
+        ensures  |clocks| <= 1
     {
         var rest;
         recvs, rest := RemoveRecvs(events);
@@ -160,14 +183,14 @@ module Host_i refines Host_s {
     }
 
     lemma NetEventsRespectReduction(s:Node, s':Node, ios:seq<LockIo>, events:seq<NetEvent>)
-        requires LIoOpSeqCompatibleWithReduction(ios);
-        requires AbstractifyRawLogToIos(events) == ios;
-        ensures NetEventsReductionCompatible(events);
+        requires LIoOpSeqCompatibleWithReduction(ios)
+        requires AbstractifyRawLogToIos(events) == ios
+        ensures NetEventsReductionCompatible(events)
     {
         //reveal_AbstractifyRawLogToIos();
         assert AbstractifyRawLogToIos(events) == ios;
         forall i | 0 <= i < |events| - 1 
-            ensures events[i].LIoOpReceive? || events[i+1].LIoOpSend?;
+            ensures events[i].LIoOpReceive? || events[i+1].LIoOpSend?
         {
             assert AbstractifyRawLogToIos(events)[i] == ios[i];
             assert AbstractifyRawLogToIos(events)[i+1] == ios[i+1];
@@ -178,6 +201,21 @@ module Host_i refines Host_s {
         returns (ok:bool, host_state':HostState, 
                  ghost recvs:seq<NetEvent>, ghost clocks:seq<NetEvent>, ghost sends:seq<NetEvent>, 
                  ghost ios:seq<LIoOp<EndPoint, seq<byte>>>)
+        requires env.Valid() && env.ok.ok()
+        requires HostStateInvariants(host_state, env)
+        modifies set x:object | ArbitraryObject(x)     // Everything!
+        ensures  ok <==> env.Valid() && env.ok.ok()
+        ensures  ok ==> HostStateInvariants(host_state', env)
+        ensures  ok ==> HostNext(host_state, host_state', ios)
+        // Connect the low-level IO events to the spec-level IO events
+        ensures  ok ==> recvs + clocks + sends == ios
+        // These obligations enable us to apply reduction
+        // Even when !ok, if sent is non-empty, we need to return valid set of sent packets too
+        ensures  (ok || |sends| > 0) ==> env.net.history() == old(env.net.history()) + (recvs + clocks + sends)
+        ensures  forall e :: && (e in recvs ==> e.LIoOpReceive?) 
+                        && (e in clocks ==> e.LIoOpReadClock? || e.LIoOpTimeoutReceive?) 
+                        && (e in sends ==> e.LIoOpSend?)
+        ensures  |clocks| <= 1
     {
         var okay, netEventLog, abstract_ios := host_state.node_impl.HostNextMain();
         if okay {
